src/Parsers/Reachable/AllReachable.v
@@ -15,7 +15,7 @@ Section cfg.
   Context (ch : Char).
 
   (** Relation defining if a character is reachable *)
-  Inductive reachable_from_productions : productions Char -> Prop :=
+  Inductive reachable_from_productions : productions Char -> Type :=
   | ReachableHead : forall pat pats, reachable_from_production pat
                                      -> reachable_from_productions (pat::pats)
   | ReachableTail : forall pat pats, reachable_from_productions pats
@@ -25,7 +25,7 @@ Section cfg.
                                              -> reachable_from_production (it::its)
   | ReachableProductionTail : forall it its, reachable_from_production its
                                              -> reachable_from_production (it::its)
-  with reachable_from_item : item Char -> Prop :=
+  with reachable_from_item : item Char -> Type :=
   | ReachableTerminal : reachable_from_item (Terminal ch)
   | ReachableNonTerminal : forall nt, is_valid_nonterminal initial_nonterminals_data nt
                                       -> reachable_from_productions (Lookup G nt)
