src/Parsers/BaseTypesLemmas.v
@@ -1,0 +1,125 @@
+(** * Lemmas about the common part of the interface of the CFG parser *)
+Require Import Coq.Classes.RelationClasses Coq.Setoids.Setoid.
+Require Import Coq.Lists.List Coq.Arith.Wf_nat Coq.Init.Wf Coq.Strings.String.
+Require Import Fiat.Parsers.ContextFreeGrammar.
+Require Import Fiat.Parsers.BaseTypes.
+
+Set Implicit Arguments.
+
+Local Open Scope string_like_scope.
+
+Local Coercion is_true : bool >-> Sortclass.
+
+Section recursive_descent_parser.
+  Context {Char} {HSL : StringLike Char} {G : grammar Char}
+          {predata : parser_computational_predataT}
+          {rdata' : parser_removal_dataT'}.
+
+  Lemma remove_nonterminal_3
+        {ls ps ps'} (H0 : is_valid_nonterminal ls ps = false)
+  : is_valid_nonterminal (remove_nonterminal ls ps) ps' = is_valid_nonterminal ls ps'.
+  Proof.
+    case_eq (is_valid_nonterminal (remove_nonterminal ls ps) ps');
+    case_eq (is_valid_nonterminal ls ps');
+    intros H' H'';
+    try reflexivity;
+    exfalso;
+    first [ apply remove_nonterminal_1 in H''
+          | apply remove_nonterminal_2 in H''; destruct H''; subst ];
+    congruence.
+  Qed.
+
+  Lemma remove_nonterminal_4
+        {ls ps ps'} (H0 : is_valid_nonterminal (remove_nonterminal ls ps) ps')
+  : ps <> ps'.
+  Proof.
+    intro H'.
+    pose proof (proj2 (remove_nonterminal_2 ls _ _) (or_intror H')).
+    congruence.
+  Qed.
+
+  Lemma remove_nonterminal_5
+        {ls ps ps'} (H0 : ps <> ps')
+  : is_valid_nonterminal (remove_nonterminal ls ps) ps' = is_valid_nonterminal ls ps'.
+  Proof.
+    case_eq (is_valid_nonterminal (remove_nonterminal ls ps) ps');
+    case_eq (is_valid_nonterminal ls ps');
+    intros H' H'';
+    try reflexivity;
+    exfalso;
+    first [ apply remove_nonterminal_1 in H''
+          | apply remove_nonterminal_2 in H''; destruct H''; subst ];
+    congruence.
+  Qed.
+
+  Lemma remove_nonterminal_6
+        ls ps
+  : is_valid_nonterminal (remove_nonterminal ls ps) ps = false.
+  Proof.
+    apply remove_nonterminal_2; right; reflexivity.
+  Qed.
+
+  Global Instance sub_nonterminals_listT_Reflexive : Reflexive sub_nonterminals_listT
+    := fun x y f => f.
+
+  Global Instance sub_nonterminals_listT_Transitive : Transitive sub_nonterminals_listT.
+  Proof.
+    lazy; auto.
+  Defined.
+
+  Global Add Parametric Morphism : remove_nonterminal
+  with signature sub_nonterminals_listT ==> eq ==> sub_nonterminals_listT
+    as remove_nonterminal_mor.
+  Proof.
+    intros x y H0 z w H'.
+    hnf in H0.
+    pose proof (remove_nonterminal_4 H').
+    apply remove_nonterminal_1 in H'.
+    rewrite remove_nonterminal_5 by assumption.
+    auto.
+  Qed.
+
+  Lemma sub_nonterminals_listT_remove ls ps
+  : sub_nonterminals_listT (remove_nonterminal ls ps) ls.
+  Proof.
+    intros p.
+    apply remove_nonterminal_1.
+  Qed.
+
+  Lemma sub_nonterminals_listT_remove_2 {ls ls' ps} (H : sub_nonterminals_listT ls ls')
+  : sub_nonterminals_listT (remove_nonterminal ls ps) ls'.
+  Proof.
+    etransitivity; eauto using sub_nonterminals_listT_remove.
+  Qed.
+
+  Lemma sub_nonterminals_listT_remove_3 {ls ls' p}
+        (H0 : is_valid_nonterminal ls p = false)
+        (H1 : sub_nonterminals_listT ls ls')
+  : sub_nonterminals_listT ls (remove_nonterminal ls' p).
+  Proof.
+    intros p' H'.
+    rewrite remove_nonterminal_5; intuition (subst; eauto; congruence).
+  Qed.
+
+  Lemma remove_nonterminal_noninc' {ls nt}
+  : nonterminals_length (remove_nonterminal ls nt) <= nonterminals_length ls.
+  Proof.
+    apply NPeano.Nat.nlt_ge.
+    apply remove_nonterminal_noninc.
+  Qed.
+
+  Lemma nonempty_nonterminals {ls nt} (H : is_valid_nonterminal ls nt)
+  : 0 < nonterminals_length ls.
+  Proof.
+    eapply Lt.le_lt_trans;
+    [ apply Le.le_0_n
+    | exact (remove_nonterminal_dec ls nt H) ].
+  Qed.
+
+  Lemma nonempty_nonterminals' {ls nt} (H : is_valid_nonterminal ls nt)
+  : negb (EqNat.beq_nat (nonterminals_length ls) 0).
+  Proof.
+    pose proof (nonempty_nonterminals H).
+    destruct (nonterminals_length ls); simpl; try reflexivity; try omega.
+  Qed.
+End recursive_descent_parser.
