src/Parsers/Reachable/AllMinimalReachable.v
@@ -1,0 +1,35 @@
+(** * Definition of minimal parse trees *)
+Require Import Coq.Strings.String Coq.Lists.List Coq.Setoids.Setoid.
+Require Import Fiat.Parsers.ContextFreeGrammar.
+Require Import Fiat.Parsers.Reachable.AllReachable.
+Require Import Fiat.Parsers.BaseTypes.
+
+Local Coercion is_true : bool >-> Sortclass.
+
+Set Implicit Arguments.
+Local Open Scope string_like_scope.
+
+Section cfg.
+  Context {Char} {HSL : StringLike Char} {G : grammar Char}.
+  Context {predata : @parser_computational_predataT}
+          {rdata' : @parser_removal_dataT' predata}.
+
+  Context (ch : Char).
+
+  Inductive minimal_reachable_from_productions : nonterminals_listT -> productions Char -> Type :=
+  | MinReachableHead : forall valid pat pats, minimal_reachable_from_production valid pat
+                                              -> minimal_reachable_from_productions valid (pat::pats)
+  | MinReachableTail : forall valid pat pats, minimal_reachable_from_productions valid pats
+                                              -> minimal_reachable_from_productions valid (pat::pats)
+  with minimal_reachable_from_production : nonterminals_listT -> production Char -> Type :=
+  | MinReachableProductionHead : forall valid it its, minimal_reachable_from_item valid it
+                                                      -> minimal_reachable_from_production valid (it::its)
+  | MinReachableProductionTail : forall valid it its, minimal_reachable_from_production valid its
+                                                      -> minimal_reachable_from_production valid (it::its)
+  with minimal_reachable_from_item : nonterminals_listT -> item Char -> Type :=
+  | MinReachableTerminal : forall valid, minimal_reachable_from_item valid (Terminal ch)
+  | MinReachableNonTerminal : forall valid nt, is_valid_nonterminal valid nt
+                                               -> minimal_reachable_from_productions (remove_nonterminal valid nt) (Lookup G nt)
+                                               -> minimal_reachable_from_item valid (NonTerminal nt).
+
+End cfg.
