src/Parsers/Reachable/AllMinimalReachableOfReachable.v
@@ -1,0 +1,635 @@
+(** * Every parse tree has a corresponding minimal parse tree *)
+Require Import Coq.Program.Basics.
+Require Import Coq.Strings.String Coq.Lists.List Coq.Setoids.Setoid Coq.Classes.RelationClasses Coq.Classes.Morphisms.
+Require Import Fiat.Parsers.ContextFreeGrammar.
+Require Import Fiat.Parsers.Reachable.AllReachable.
+Require Import Fiat.Parsers.Reachable.AllMinimalReachable.
+Require Import Fiat.Parsers.BaseTypes.
+Require Import Fiat.Parsers.BaseTypesLemmas.
+Require Import Fiat.Parsers.Reachable.AllReachableWellFounded.
+Require Import Fiat.Common.
+(*Require Import Coq.Strings.String Coq.Lists.List Coq.Program.Program Coq.Classes.RelationClasses Coq.Classes.Morphisms Coq.Setoids.Setoid Coq.Arith.Compare_dec.
+Require Import Coq.omega.Omega.
+Require Import Coq.Program.Wf Coq.Arith.Wf_nat.
+Require Import Fiat.Parsers.ContextFreeGrammar Fiat.Parsers.ContextFreeGrammarProperties Fiat.Parsers.WellFoundedParse.
+Require Import Fiat.Parsers.CorrectnessBaseTypes Fiat.Parsers.BaseTypes.
+Require Export Fiat.Parsers.MinimalParse.
+Require Export Fiat.Parsers.WellFoundedParseProperties.
+Require Import Fiat.Common Fiat.Common.Le Fiat.Common.Wf.*)
+
+Set Implicit Arguments.
+Local Open Scope string_like_scope.
+
+Section cfg.
+  Context {Char} {HSL : StringLike Char} {HSLP : StringLikeProperties Char} {G : grammar Char}.
+  Context {predata : parser_computational_predataT}
+          {rdata' : @parser_removal_dataT' predata}.
+
+  Definition reachable_from_item__of__minimal_reachable_from_item'
+             {ch}
+             (reachable_from_productions__of__minimal_reachable_from_productions
+              : forall valid prods,
+                  sub_nonterminals_listT valid initial_nonterminals_data
+                  -> minimal_reachable_from_productions (G := G) ch valid prods
+                  -> reachable_from_productions G ch prods)
+             valid it
+             (Hsub : sub_nonterminals_listT valid initial_nonterminals_data)
+             (H : minimal_reachable_from_item (G := G) ch valid it)
+  : reachable_from_item G ch it.
+  Proof.
+    destruct H; [ left | right ].
+    { clear reachable_from_productions__of__minimal_reachable_from_productions; eauto. }
+    { eapply reachable_from_productions__of__minimal_reachable_from_productions; [ | eassumption ].
+      clear -Hsub rdata'.
+      eauto using sub_nonterminals_listT_remove_2. }
+  Defined.
+
+  Fixpoint reachable_from_productions__of__minimal_reachable_from_productions
+             {ch}
+             valid pats
+             (Hsub : sub_nonterminals_listT valid initial_nonterminals_data)
+             (H : minimal_reachable_from_productions (G := G) ch valid pats)
+  : reachable_from_productions G ch pats
+  with reachable_from_production__of__minimal_reachable_from_production
+             {ch}
+             valid pat
+             (Hsub : sub_nonterminals_listT valid initial_nonterminals_data)
+             (H : minimal_reachable_from_production (G := G) ch valid pat)
+  : reachable_from_production G ch pat.
+  Proof.
+    { destruct H; [ left | right ]; eauto. }
+    { destruct H; [ left | right ]; eauto using reachable_from_item__of__minimal_reachable_from_item'. }
+  Defined.
+
+  Definition reachable_from_item__of__minimal_reachable_from_item
+             {ch}
+    := @reachable_from_item__of__minimal_reachable_from_item' ch reachable_from_productions__of__minimal_reachable_from_productions.
+
+  Section expand.
+    Definition expand_minimal_reachable_from_item'
+               {ch}
+               (expand_minimal_reachable_from_productions
+                : forall valid valid' prods,
+                    sub_nonterminals_listT valid valid'
+                    -> minimal_reachable_from_productions (G := G) ch valid prods
+                    -> minimal_reachable_from_productions (G := G) ch valid' prods)
+               valid valid' it
+               (Hsub : sub_nonterminals_listT valid valid')
+               (H : minimal_reachable_from_item (G := G) ch valid it)
+    : minimal_reachable_from_item (G := G) ch valid' it.
+    Proof.
+      destruct H; [ left | right ].
+      { clear expand_minimal_reachable_from_productions; eauto. }
+      { eapply expand_minimal_reachable_from_productions; [ | eassumption ].
+        clear -Hsub rdata'.
+        eauto using remove_nonterminal_mor. }
+    Defined.
+
+    Fixpoint expand_minimal_reachable_from_productions
+             {ch}
+             valid valid' pats
+             (Hsub : sub_nonterminals_listT valid valid')
+             (H : minimal_reachable_from_productions (G := G) ch valid pats)
+    : minimal_reachable_from_productions (G := G) ch valid' pats
+    with expand_minimal_reachable_from_production
+           {ch}
+           valid valid' pat
+           (Hsub : sub_nonterminals_listT valid valid')
+           (H : minimal_reachable_from_production (G := G) ch valid pat)
+         : minimal_reachable_from_production (G := G) ch valid' pat.
+    Proof.
+      { destruct H; [ left | right ]; eauto. }
+      { destruct H; [ left | right ]; eauto using expand_minimal_reachable_from_item'. }
+    Defined.
+
+    Definition expand_minimal_reachable_from_item
+               {ch}
+      := @expand_minimal_reachable_from_item' ch expand_minimal_reachable_from_productions.
+  End expand.
+
+  (*Global Instance minimal_reachable_from_item_Proper {ch}
+  : Proper (sub_nonterminals_listT ==> eq ==> impl) (minimal_reachable_from_item (G := G) ch).
+  Proof. repeat intro; subst; eapply expand_minimal_reachable_from_item; eauto. Qed.
+
+  Global Instance minimal_reachable_from_production_Proper {ch}
+  : Proper (sub_nonterminals_listT ==> eq ==> impl) (minimal_reachable_from_production (G := G) ch).
+  Proof. repeat intro; subst; eapply expand_minimal_reachable_from_production; eauto. Qed.
+
+  Global Instance minimal_reachable_from_productions_Proper {ch}
+  : Proper (sub_nonterminals_listT ==> eq ==> impl) (minimal_reachable_from_productions (G := G) ch).
+  Proof. repeat intro; subst; eapply expand_minimal_reachable_from_productions; eauto. Qed.*)
+
+  Section minimize.
+    Context {ch : Char}.
+
+    Let alt_option h valid
+      := { nt : _ & (is_valid_nonterminal valid nt = false /\ is_valid_nonterminal initial_nonterminals_data nt)
+                    * { p : reachable_from_productions G ch (Lookup G nt)
+                            & (size_of_reachable_from_productions p < h) } }%type.
+
+    Lemma not_alt_all {h} (ps : alt_option h initial_nonterminals_data)
+    : False.
+    Proof.
+      destruct ps as [ ? [ H' _ ] ].
+      revert H'; clear; intros [? ?].
+      congruence.
+    Qed.
+
+    Definition alt_all_elim {h T} (ps : T + alt_option h initial_nonterminals_data)
+    : T.
+    Proof.
+      destruct ps as [|ps]; [ assumption | exfalso ].
+      eapply not_alt_all; eassumption.
+    Defined.
+
+    Definition expand_alt_option' {h h' valid valid'}
+               (H : h <= h') (H' : sub_nonterminals_listT valid' valid)
+    : alt_option h valid -> alt_option h' valid'.
+    Proof.
+      hnf in H'; unfold alt_option.
+      repeat match goal with
+               | [ |- sigT _ -> _ ] => intros []
+               | [ |- sig _ -> _ ] => intros []
+               | [ |- prod _ _ -> _ ] => intros []
+               | [ |- and _ _ -> _ ] => intros []
+               | _ => intro
+               | _ => progress subst
+               | [ |- sigT _ ] => esplit
+               | [ |- sig _ ] => esplit
+               | [ |- prod _ _ ] => split
+               | [ |- and _ _ ] => split
+               | [ H : _ = false |- _ = false ]
+                 => apply Bool.not_true_iff_false in H;
+                   apply Bool.not_true_iff_false;
+                   intro; apply H
+               | _ => eapply H'; eassumption
+               | _ => assumption
+               | [ |- _ < _ ] => eapply Lt.lt_trans; eassumption
+               | [ |- _ < _ ] => eapply Lt.lt_le_trans; eassumption
+             end.
+    Defined.
+
+    Definition expand_alt_option {h h' valid valid'}
+               (H : h < h') (H' : sub_nonterminals_listT valid' valid)
+    : alt_option h valid -> alt_option h' valid'.
+    Proof.
+      apply expand_alt_option'; try assumption.
+      apply Lt.lt_le_weak; assumption.
+    Defined.
+
+    Section wf_parts.
+      Let of_item_T' h
+          (valid : nonterminals_listT) {it : item Char}
+          (p : reachable_from_item G ch it)
+        := forall (p_small : size_of_reachable_from_item p < h)
+                  (pf : sub_nonterminals_listT valid initial_nonterminals_data),
+             ({ p' : minimal_reachable_from_item (G := G) ch valid it
+                     & (size_of_reachable_from_item (reachable_from_item__of__minimal_reachable_from_item pf p')) <= size_of_reachable_from_item p })%type
+             + alt_option (size_of_reachable_from_item p) valid.
+
+      Let of_item_T h
+        := forall valid it p, @of_item_T' h valid it p.
+
+      Let of_parse_production_T' h
+          (valid : nonterminals_listT) {pat : production Char}
+          (p : reachable_from_production G str pat)
+        := forall (p_small : size_of_parse_production p < h),
+             sub_nonterminals_listT valid initial_nonterminals_data
+             -> Forall_reachable_from_production P p
+             -> ({ p' : minimal_reachable_from_production (G := G) len0 valid pat
+                        & (size_of_parse_production (projT1 (reachable_from_production__of__minimal_reachable_from_production p')) <= size_of_parse_production p)
+                          * Forall_reachable_from_production P (projT1 (reachable_from_production__of__minimal_reachable_from_production p')) })%type
+                + alt_option (size_of_parse_production p) valid.
+
+      Let of_parse_production_T len0 h
+        := forall str pf valid pat p, @of_parse_production_T' h len0 str pf valid pat p.
+
+      Let of_parse_T' h
+          {len0} {str : String} (pf : length str <= len0)
+          (valid : nonterminals_listT) {pats : productions Char}
+          (p : parse_of G str pats)
+        := forall (p_small : size_of_parse p < h),
+             sub_nonterminals_listT valid initial_nonterminals_data
+             -> Forall_parse_of P p
+             -> ({ p' : minimal_parse_of (G := G) len0 valid pats
+                        & (size_of_parse (projT1 (parse_of__of__minimal_parse_of p')) <= size_of_parse p)
+                          * Forall_parse_of P (projT1 (parse_of__of__minimal_parse_of p')) })%type
+                + alt_option (size_of_parse p) valid.
+
+      Let of_parse_T len0 h
+        := forall str pf valid pats p, @of_parse_T' h len0 str pf valid pats p.
+
+      Let of_parse_nonterminal_T {len0 str valid nonterminal} (p : parse_of G str (Lookup G nonterminal)) h
+        := size_of_reachable_from_item (ParseNonTerminal nonterminal p) < h
+           -> length str <= len0
+           -> sub_nonterminals_listT valid initial_nonterminals_data
+           -> Forall_reachable_from_item P (ParseNonTerminal nonterminal p)
+           -> ({ p' : minimal_parse_of_nonterminal (G := G) len0 valid nonterminal
+                      & (size_of_reachable_from_item (projT1 (reachable_from_item__of__minimal_reachable_from_item (MinParseNonTerminal p'))) <= size_of_reachable_from_item (ParseNonTerminal nonterminal p))
+                        * Forall_reachable_from_item P (projT1 (reachable_from_item__of__minimal_reachable_from_item (MinParseNonTerminal p'))) })%type
+              + alt_option (size_of_reachable_from_item (ParseNonTerminal nonterminal p)) valid.
+
+      Section item.
+        Context {len0 : nat} {str : String} {valid : nonterminals_listT}.
+
+        Definition minimal_reachable_from_item__of__reachable_from_item
+                   h
+                   (minimal_parse_of_nonterminal__of__parse_of_nonterminal
+                    : forall h' (pf : h' < S (S h)) {len0 str valid nonterminal}
+                             (p : parse_of G str (Lookup G nonterminal)),
+                        @of_parse_nonterminal_T len0 str valid nonterminal p h')
+        : of_item_T len0 h.
+        Proof.
+          intros str' pf valid' pats p H_h Hinit' H_forall.
+          destruct h as [|h']; [ exfalso; omega | ].
+          destruct p as [ ch pf0 |nonterminal' p'].
+          { left.
+            eexists (MinimalParse.MinParseTerminal _ _ _ _ pf0);
+              split; simpl; constructor. }
+          { edestruct (fun pf => @minimal_parse_of_nonterminal__of__parse_of_nonterminal (S h') pf len0 _ valid' _ p') as [ [p'' H''] | p'' ];
+            try solve [ repeat (apply Lt.lt_n_Sn || apply Lt.lt_S)
+                      | exact Hinit'
+                      | exact H_h
+                      | exact H_forall
+                      | exact pf ];
+            [|];
+            [ left | right ].
+            { exists (MinParseNonTerminal p'').
+              simpl in *.
+              exact H''. }
+            { exact p''. } }
+        Defined.
+      End item.
+
+      Section production.
+        Context {len0 : nat} {str : String} {valid : nonterminals_listT}.
+
+        Local Ltac min_parse_prod_t' :=
+          idtac;
+          match goal with
+            | _ => assumption
+            | [ |- ?R ?x ?x ]
+              => reflexivity
+            | _ => progress destruct_head prod
+            | [ H : False |- _ ]
+              => solve [ destruct H ]
+            | _ => progress simpl
+            | _ => progress subst
+            | _ => progress rewrite ?parse_of_contract_minimal_reachable_from_item_lt, ?parse_of_contract_minimal_reachable_from_production_lt, ?parse_of_contract_minimal_parse_of_lt
+            | [ |- context G[size_of_parse_production (ParseProductionCons ?s ?n ?a ?b)] ]
+              => let G' := context G[S (size_of_reachable_from_item a + size_of_parse_production b)] in
+                 change G'
+            | [ H : alt_option _ initial_nonterminals_data _ |- _ ]
+              => apply not_alt_all in H
+            | [ p0 : minimal_reachable_from_item ?ns' ?v (take ?n ?s) ?pat,
+                     p1 : minimal_reachable_from_production ?ns' ?v (drop ?n ?s) ?pats,
+                          H : length ?s <= ?ns'
+                |- ({ p' : minimal_reachable_from_production ?ns' ?v ?s (?pat :: ?pats) & _ } + _)%type ]
+              => left; exists (MinParseProductionCons _ n H p0 p1)
+            | [ p0 : minimal_reachable_from_item ?ns' _ (take ?n ?s) ?pat,
+                     p1 : minimal_reachable_from_production ?ns' ?v (drop ?n ?s) ?pats,
+                          H : length ?s <= ?ns'
+                |- ({ p' : minimal_reachable_from_production ?ns' ?v ?s (?pat :: ?pats) & _ } + _)%type ]
+              => let H' := fresh in
+                 assert (H' : length (take n s) < ns')
+                   by (rewrite <- H, ?take_short_length by omega; omega);
+                   left; exists (MinParseProductionCons
+                                   _
+                                   n
+                                   H
+                                   (contract_minimal_reachable_from_item_lt (valid' := v) H' p0)
+                                   p1)
+            | [ p0 : minimal_reachable_from_item ?ns' ?v (take ?n ?s) ?pat,
+                     p1 : minimal_reachable_from_production ?ns' _ (drop ?n ?s) ?pats,
+                          H : length ?s <= ?ns'
+                |- ({ p' : minimal_reachable_from_production ?ns' ?v ?s (?pat :: ?pats) & _ } + _)%type ]
+              => let H' := fresh in
+                 assert (H' : length (drop n s) < ns')
+                   by (rewrite <- H, drop_length; omega);
+                   left; exists (MinParseProductionCons
+                                   _
+                                   n
+                                   H
+                                   p0
+                                   (contract_minimal_reachable_from_production_lt (valid' := v) H' p1))
+            | [ p0 : minimal_reachable_from_item ?ns' _ (take ?n ?s) ?pat,
+                     p1 : minimal_reachable_from_production ?ns' _ (drop ?n ?s) ?pats,
+                          H : length ?s <= ?ns',
+                              H' : ?n < length ?s,
+                                   H'' : 0 < ?n
+                |- ({ p' : minimal_reachable_from_production ?ns' ?v ?s (?pat :: ?pats) & _ } + _)%type ]
+              => let H0' := fresh in
+                 let H1' := fresh in
+                 assert (H1' : length (drop n s) < ns')
+                   by (rewrite <- H, drop_length; omega);
+                   assert (H0' : length (take n s) < ns')
+                   by (rewrite <- H, ?take_short_length by omega; omega);
+                   left; eexists (MinParseProductionCons
+                                    _
+                                    n
+                                    H
+                                    (contract_minimal_reachable_from_item_lt (valid' := v) H0' p0)
+                                    (contract_minimal_reachable_from_production_lt (valid' := v) H1' p1))
+            | [ |- (_ * _)%type ]
+              => split
+            | [ H : _ <= _ |- _ <= _ ] => apply H
+            | _ => apply Le.le_n_S
+            | _ => apply Plus.plus_le_compat
+            | [ H0 : Forall_reachable_from_item _ _,
+                     H1 : Forall_reachable_from_production _ _
+                |- Forall_reachable_from_production _ _ ]
+              => exact (H0, H1)
+            | [ H : alt_option _ ?v (drop 0 ?x)
+                |- (_ + alt_option _ ?v ?x)%type ]
+              => right; eapply expand_alt_option'; [ .. | exact H ]
+            | [ H : alt_option _ ?v (drop ?n ?x), H' : length ?x <= ?n
+                |- (_ + alt_option _ ?v ?x)%type ]
+              => right; eapply expand_alt_option'; [ .. | exact H ]
+            | [ H : alt_option _ ?v (take ?n ?x), H' : length ?x = ?n
+                |- (_ + alt_option _ ?v ?x)%type ]
+              => right; eapply expand_alt_option'; [ .. | exact H ]
+            | [ H : alt_option _ ?v (take ?n ?x), H' : length ?x <= ?n
+                |- (_ + alt_option _ ?v ?x)%type ]
+              => right; eapply expand_alt_option'; [ .. | exact H ]
+            (*| [ H : alt_option _ ?v ?x
+                |- (_ + alt_option _ ?v (Empty _ ++ ?x))%type ]
+              => right; eapply expand_alt_option'; [ .. | exact H ]*)
+            (*| [ |- _ = _ ]
+              => progress rewrite ?LeftId, ?RightId*)
+            | [ H : length ?s = 0 |- beq _ ?s ] => apply bool_eq_empty
+            | [ H : length ?s = 0 |- beq ?s _ ] => apply bool_eq_empty
+            | _ => rewrite take_short_length by assumption
+            | _ => rewrite take_long by assumption
+            | [ H : context[min _ _] |- _ ] => rewrite min_l in H by assumption
+            | [ H : context[min _ _] |- _ ] => rewrite min_r in H by assumption
+            | [ H : context[min _ _] |- _ ] => rewrite min_l in H by omega
+            | [ H : context[min _ _] |- _ ] => rewrite min_r in H by omega
+            | _ => rewrite drop_length
+            | _
+              => solve [ eauto using le_S, Le.le_trans, Plus.le_plus_l, Plus.le_plus_r, drop_0, take_long, NPeano.Nat.eq_le_incl, bool_eq_empty, drop_length, (fun x y => proj2 (NPeano.Nat.sub_0_le x y)) with nocore ]
+          end.
+        (*Local Ltac min_parse_prod_pose_t' :=
+          idtac;
+          match goal with
+            | [ H : ?a <> Empty _,
+                    H' : ?a ++ _ ≤s _ |- _ ]
+              => unique pose proof (strle_to_lt_nonempty_r H H')
+            | [ H : ?a <> Empty _,
+                    H' : _ ++ ?a ≤s _ |- _ ]
+              => unique pose proof (strle_to_lt_nonempty_l H H')
+          end.*)
+        (*Local Ltac min_parse_prod_pose_t := repeat min_parse_prod_pose_t'.*)
+        Local Ltac min_parse_prod_t := repeat min_parse_prod_t'.
+
+        (** This is the proof where we pay the proof for conceptual
+            mismatch.  We are, conceptually, simultaneously
+            "minimizing parse trees" and "producing parse traces".  It
+            is marginally nicer(!!) to contain the ugliness in this
+            single proof, rather than have it infect everything.  So
+            we must conceptually minimize the passed parse tree while
+            in fact building a trace of the parse algorithm.  To do
+            this, in the cons case, we need to figure out how we're
+            decreasing.  According with conceptual minimization, when
+            we have parsed [s0 ++ s1] as a cons of [p0] and [p1],
+            having a smaller parse tree for, say [s0], with any other
+            pattern, does us no good, unless [s1] is empty (and [s0 =
+            s0 ++ s1]), when we can simply pass that smaller parse up
+            the function call tree.  So we must eliminate the
+            "alternate" option, by expanding the valid list to the
+            initial data.  Luckily(?!), in the case where [s1] is
+            non-empty, [s0] is strictly smaller than [s0 ++ s1], and
+            thus we can rebuild the minimal parse tree to contract it.
+            This, finally, allows us to either build a minimal parse
+            tree for the thing we are asked about (or to contract the
+            "alternate option" parse tree, passing it back up?). *)
+
+        Fixpoint minimal_reachable_from_production__of__reachable_from_production
+                 h
+                 (minimal_parse_of_nonterminal__of__parse_of_nonterminal
+                  : forall h' (pf : h' < S (S h)) {len0 str valid nonterminal}
+                           (p : parse_of G str (Lookup G nonterminal)),
+                      @of_parse_nonterminal_T len0 str valid nonterminal p h')
+                 {struct h}
+        : of_parse_production_T len0 h.
+        Proof.
+          intros str' pf valid' pats p H_h Hinit' H_forall.
+          destruct h as [|h']; [ exfalso; omega | ].
+          destruct p as [ pf0' | n pat' pats' p0' p1' ].
+          { clear minimal_reachable_from_production__of__reachable_from_production.
+            left.
+            eexists (@MinimalParse.MinParseProductionNil _ _ _ _ _ _ _ pf0');
+              repeat (reflexivity || esplit). }
+          { specialize (fun h' pf
+                        => @minimal_parse_of_nonterminal__of__parse_of_nonterminal
+                             h' (transitivity pf (Lt.lt_n_Sn _))).
+            change (S ((size_of_reachable_from_item p0')
+                       + (size_of_parse_production p1'))
+                    < S h') in H_h.
+            apply Lt.lt_S_n in H_h.
+            pose proof (Lt.le_lt_trans _ _ _ (Plus.le_plus_l _ _) H_h) as H_h0.
+            pose proof (Lt.le_lt_trans _ _ _ (Plus.le_plus_r _ _) H_h) as H_h1.
+            clear H_h.
+            assert (pf0' : length (take n str') <= length str')
+              by (rewrite take_length; apply Min.min_case_strong; omega).
+            assert (pf1' : length (drop n str') <= length str')
+              by (rewrite drop_length; omega).
+            pose proof (fun valid Hinit => @minimal_reachable_from_item__of__reachable_from_item _ h'  minimal_parse_of_nonterminal__of__parse_of_nonterminal _ (transitivity pf0' pf) valid _ p0' H_h0 Hinit (fst H_forall)) as p_it.
+            pose proof (fun valid Hinit => @minimal_reachable_from_production__of__reachable_from_production h' minimal_parse_of_nonterminal__of__parse_of_nonterminal _ (transitivity pf1' pf) valid _ p1' H_h1 Hinit (snd H_forall)) as p_prod.
+            clear pf0' pf1'.
+            destruct (le_lt_dec (length str') n) as [ Hle | Hle ], (zerop (min n (length str'))) as [Hstr' | Hstr' ].
+            { (* empty, empty *)
+              rewrite Min.min_r in Hstr' by assumption.
+              specialize (p_it valid' Hinit'); specialize (p_prod valid' Hinit').
+              destruct p_it as [ [ p0'' H0''] |], p_prod as [ [ p1'' H1'' ] |];
+                [ | | | ];
+                min_parse_prod_t. }
+            { (* nonempty, empty *)
+              specialize (p_it valid' Hinit'); specialize (p_prod initial_nonterminals_data (reflexivity _)).
+              destruct p_it as [ [ p0'' H0''] |], p_prod as [ [ p1'' H1'' ] |];
+                [ | | | ];
+                min_parse_prod_t. }
+            { (* empty, nonempty *)
+              specialize (p_it initial_nonterminals_data (reflexivity _)); specialize (p_prod valid' Hinit').
+              destruct p_it as [ [ p0'' H0''] |], p_prod as [ [ p1'' H1'' ] |];
+                [ | | | ];
+                min_parse_prod_t. }
+            { (* nonempty, nonempty *)
+              specialize (p_it initial_nonterminals_data (reflexivity _)); specialize (p_prod initial_nonterminals_data (reflexivity _)).
+              destruct p_it as [ [ p0'' H0''] |], p_prod as [ [ p1'' H1'' ] |];
+                [ | | | ];
+                min_parse_prod_t. } }
+        Defined.
+      End production.
+
+      Section productions.
+        Context {len0 : nat} {str : String} {valid : nonterminals_listT}.
+
+        Fixpoint minimal_reachable_from_productions__of__reachable_from_productions
+                 h
+                 (minimal_parse_of_nonterminal__of__parse_of_nonterminal
+                  : forall h' (pf : h' < S h) {len0 str valid nonterminal}
+                           (p : parse_of G str (Lookup G nonterminal)),
+                      @of_parse_nonterminal_T len0 str valid nonterminal p h')
+                 {struct h}
+        : of_parse_T len0 h.
+        Proof.
+          intros str' pf valid' pats p H_h Hinit' H_forall.
+          destruct h as [|h']; [ exfalso; omega | ].
+          destruct p as [pat pats p' | pat pats p'].
+          { clear minimal_reachable_from_productions__of__reachable_from_productions.
+            edestruct (@minimal_reachable_from_production__of__reachable_from_production _ h' minimal_parse_of_nonterminal__of__parse_of_nonterminal _ pf valid' _ p') as [ [p'' p''H] | [nonterminal' H'] ];
+            try solve [ exact (Lt.lt_S_n _ _ H_h)
+                      | exact H_forall
+                      | exact Hinit' ];
+            [|].
+            { left.
+              exists (MinParseHead pats p'').
+              simpl.
+              split;
+                solve [ exact (Le.le_n_S _ _ (fst p''H))
+                      | exact (snd p''H) ]. }
+            { right.
+              exists nonterminal'.
+              split;
+                try solve [ exact (fst H') ];
+                [].
+              exists (projT1 (snd H'));
+                split;
+                try solve [ exact (snd (projT2 (snd H')))
+                          | exact (Lt.lt_S _ _ (fst (projT2 (snd H')))) ]. } }
+          { specialize (fun h' pf
+                        => @minimal_parse_of_nonterminal__of__parse_of_nonterminal
+                             h' (transitivity pf (Lt.lt_n_Sn _))).
+            edestruct (minimal_reachable_from_productions__of__reachable_from_productions h'  minimal_parse_of_nonterminal__of__parse_of_nonterminal _ pf valid' _ p') as [ [p'' p''H] | [nonterminal' H'] ];
+            try solve [ exact (Lt.lt_S_n _ _ H_h)
+                      | exact Hinit'
+                      | exact H_forall ];
+            [|].
+            { left.
+              exists (MinParseTail pat p'').
+              simpl.
+              split;
+                solve [ exact (Le.le_n_S _ _ (fst p''H))
+                      | exact (snd p''H) ]. }
+            { right.
+              exists nonterminal'.
+              split;
+                try solve [ exact (fst H') ];
+                [].
+              exists (projT1 (snd H'));
+                split;
+                try solve [ exact (snd (projT2 (snd H')))
+                          | exact (Lt.lt_S _ _ (fst (projT2 (snd H')))) ]. } }
+        Defined.
+      End productions.
+
+      Section nonterminal.
+        Section step.
+          Definition minimal_parse_of_nonterminal__of__parse_of_nonterminal_step
+                     h
+                     (minimal_parse_of_nonterminal__of__parse_of_nonterminal
+                      : forall h' (pf : h' < h) {len0 str valid nonterminal}
+                               (p : parse_of G str (Lookup G nonterminal)),
+                          @of_parse_nonterminal_T len0 str valid nonterminal p h')
+                     {len0 str valid nonterminal}
+                     (p : parse_of G str (Lookup G nonterminal))
+          : @of_parse_nonterminal_T len0 str valid nonterminal p h.
+          Proof.
+            destruct h as [|h]; [ clear; repeat intro; exfalso; omega | ].
+            intros pf Hstr Hinit' H_forall.
+            let H := match goal with H : length str <= len0 |- _ => constr:H end in
+
+            destruct (le_lt_eq_dec _ _ H) as [pf_lt|pf_eq].
+            { (** [str] got smaller, so we reset the valid nonterminals list *)
+              destruct (@minimal_reachable_from_productions__of__reachable_from_productions (length str) h minimal_parse_of_nonterminal__of__parse_of_nonterminal str (reflexivity _) initial_nonterminals_data (Lookup G nonterminal) p (Lt.lt_S_n _ _ pf) (reflexivity _) (snd H_forall)) as [p'|p'].
+              { left.
+                exists (MinParseNonTerminalStrLt valid _ pf_lt (fst H_forall) (projT1 p'));
+                  simpl.
+                simpl in *.
+                split;
+                  [ exact (Le.le_n_S _ _ (fst (projT2 p')))
+                  | split;
+                    [ exact (fst H_forall)
+                    | exact (snd (projT2 p')) ] ]. }
+              { simpl.
+                right; eapply expand_alt_option; [..| exact p' ];
+                solve [ apply Lt.lt_n_Sn
+                      | assumption
+                      | reflexivity ]. } }
+            { (** [str] didn't get smaller, so we cache the fact that we've hit this nonterminal already *)
+              destruct (Sumbool.sumbool_of_bool (is_valid_nonterminal valid nonterminal)) as [ Hvalid | Hinvalid ].
+              { destruct (@minimal_reachable_from_productions__of__reachable_from_productions len0 h minimal_parse_of_nonterminal__of__parse_of_nonterminal str Hstr (remove_nonterminal valid nonterminal) (Lookup G nonterminal) p (Lt.lt_S_n _ _ pf) (transitivity (R := sub_nonterminals_listT) (@sub_nonterminals_listT_remove _ _ _ _) Hinit') (snd H_forall)) as [p'|p'].
+                { left.
+                  exists (@MinimalParse.MinParseNonTerminalStrEq _ _ _ _ _ _ _ _ pf_eq (fst H_forall) Hvalid (projT1 p')).
+                  simpl in *.
+                  split;
+                    [ exact (Le.le_n_S _ _ (fst (projT2 p')))
+                    | split;
+                      [ exact (fst H_forall)
+                      | exact (snd (projT2 p')) ] ]. }
+                { destruct p' as [nonterminal' p'].
+                  destruct (string_dec nonterminal nonterminal') as [|n].
+                  { subst nonterminal; simpl in *.
+                    edestruct (@minimal_parse_of_nonterminal__of__parse_of_nonterminal (S (size_of_parse p)) pf len0 _ valid nonterminal' (projT1 (snd p'))) as [p''|p''];
+                    try solve [ apply Lt.lt_n_S, (fst (projT2 (snd p')))
+                              | subst; reflexivity
+                              | assumption
+                              | split; [ exact (proj2 (fst p'))
+                                       | exact (snd (projT2 (snd p'))) ] ];
+                    [|].
+                    { left.
+                      exists (projT1 p'').
+                      split.
+                      { etransitivity;
+                        [ exact (fst (projT2 p''))
+                        | exact (Lt.lt_le_weak _ _ (Lt.lt_n_S _ _ (fst (projT2 (snd p'))))) ]. }
+                      { exact (snd (projT2 p'')). } }
+                    { right.
+                      exists (projT1 p'').
+                      split;
+                        [ exact (fst (projT2 p''))
+                        | ].
+                      exists (projT1 (snd (projT2 p''))).
+                      split;
+                        [ etransitivity;
+                          [ exact (fst (projT2 (snd (projT2 p''))))
+                          | exact (Lt.lt_n_S _ _ (fst (projT2 (snd p')))) ]
+                        | exact (snd (projT2 (snd (projT2 p'')))) ]. } }
+                  { right.
+                    exists nonterminal'.
+                    destruct p' as [p'H p'p].
+                    split.
+                    { rewrite remove_nonterminal_5 in p'H by assumption.
+                      exact p'H. }
+                    { exists (projT1 p'p).
+                      split; [ exact (Lt.lt_S _ _ (fst (projT2 p'p)))
+                             | exact (snd (projT2 p'p)) ]. } } } }
+              { (** oops, we already saw this nonterminal in the past.  ABORT! *)
+                right.
+                exists nonterminal.
+                destruct H_forall.
+                split; [ split; assumption
+                       | ].
+                exists p.
+                split; solve [ assumption
+                             | apply Lt.lt_n_Sn ]. } }
+          Defined.
+        End step.
+
+        Section wf.
+          Definition minimal_parse_of_nonterminal__of__parse_of_nonterminal
+          : forall h
+                   {len0 str valid nonterminal}
+                   (p : parse_of G str (Lookup G nonterminal)),
+              @of_parse_nonterminal_T len0 str valid nonterminal p h
+            := @Fix
+                 _ lt lt_wf
+                 (fun h => forall {len0 str valid nonterminal}
+                                  (p : parse_of G str (Lookup G nonterminal)),
+                             @of_parse_nonterminal_T len0 str valid nonterminal p h)
+                 (@minimal_parse_of_nonterminal__of__parse_of_nonterminal_step).
+        End wf.
+      End nonterminal.
+    End wf_parts.
+  End minimize.
+End cfg.
